feat: prenex_normal_form

src/QL/FOL/deduction.lean
@@ -7,6 +7,12 @@ open_locale logic_symbol
 open subterm subformula logic logic.Theory
 variables {L : language.{u}} {m : ℕ}
 
+local prefix (name := mlift) `𝗟`:max := subformula.mlift
+local prefix (name := preTheory.mlift) `𝗟'`:max := preTheory.mlift
+local prefix (name := push) `𝗠`:max := subformula.push
+local prefix (name := pull) `𝗡`:max := subformula.pull
+local prefix (name := dummy) `𝗗`:max := subformula.dummy
+
 def fin.bit0 {n} : fin n → fin (bit0 n)
 | ⟨i, hi⟩ := ⟨bit0 i, by simpa using hi⟩
 
@@ -23,7 +29,7 @@ def eq_axiom5 {n} (r : L.pr n) : subformula L 0 0 :=
 ∀'*((⋀ i, #i.bit0 =' #i.bit1) ⟶ relation r (var ∘ fin.bit0) ⟶ relation r (var ∘ fin.bit1))
 
 inductive proof : Π {m}, preTheory L m → subformula L m 0 → Type u
-| generalize   {m} {T : preTheory L m} : ∀ {p}, proof T.mlift p → proof T (∀'p.pull)
+| generalize   {m} {T : preTheory L m} : ∀ {p}, proof T.mlift p → proof T (∀'𝗡p)
 | mdp          {m} {T : preTheory L m} : ∀ {p q}, proof T (p ⟶ q) → proof T p → proof T q
 | by_axiom     {m} {T : preTheory L m} : ∀ {p}, p ∈ T → proof T p
 | verum        {m} {T : preTheory L m} : proof T ⊤
@@ -32,6 +38,7 @@ inductive proof : Π {m}, preTheory L m → subformula L m 0 → Type u
 | contra       {m} {T : preTheory L m} : ∀ {p q}, proof T ((∼p ⟶ ∼q) ⟶ q ⟶ p)
 | specialize   {m} {T : preTheory L m} : ∀ {p} {t}, proof T (∀'p ⟶ subst t p)
 | dummy_univ   {m} {T : preTheory L m} : ∀ {p q}, proof T (∀'(dummy p ⟶ q) ⟶ p ⟶ ∀'q)
+| non_empty    {T : Theory L} : proof T (∃'⊤)
 | eq_refl      {T : Theory L} : proof T ∀'(#0 =' #0)
 | eq_symm      {T : Theory L} : proof T ∀' ∀'((#0 =' #1) ⟶ (#1 =' #0))
 | eq_trans     {T : Theory L} : proof T ∀' ∀' ∀'((#0 =' #1) ⟶ (#1 =' #2) ⟶ (#0 =' #2))
@@ -75,6 +82,7 @@ begin
   { intros U ss, exact contra },
   { intros U ss, exact specialize },
   { intros U ss, exact dummy_univ },
+  { intros U ss, exact non_empty },
   { intros U ss, exact eq_refl },
   { intros U ss, exact eq_symm },
   { intros U ss, exact eq_trans },
@@ -90,11 +98,19 @@ variables {T U : preTheory L m} {T₀ : Theory L}
 
 lemma generalize {p} (h : T.mlift ⊢ p) : T ⊢ ∀'p.pull := by rcases h; exact ⟨h.generalize⟩
 
+lemma generalize' {T : preTheory L (m + 1)} {p} (h : T ⊢ p) (hT : T = U.mlift) : U ⊢ ∀'p.pull :=
+by rcases hT with rfl; exact generalize h
+
+lemma gen {p : subformula L m 1} (h : T.mlift ⊢ p.push) : T ⊢ ∀'p :=
+by rw[←subformula.pull_push p]; exact generalize h
+
 lemma by_axiom {p} (h : p ∈ T) : T ⊢ p := ⟨proof.by_axiom h⟩
 
-@[simp] lemma specialize {p} (t) : T ⊢ ∀'p ⟶ subst t p := ⟨proof.specialize⟩
+@[simp] lemma specialize (p) (t) : T ⊢ ∀'p ⟶ subst t p := ⟨proof.specialize⟩
 
 @[simp] lemma dummy_univ (p q) : T ⊢ ∀'(dummy p ⟶ q) ⟶ p ⟶ ∀'q := ⟨proof.dummy_univ⟩
+
+@[simp] lemma non_empty : T₀ ⊢ ∃'⊤ := ⟨proof.non_empty⟩
 
 @[simp] lemma eq_refl : T₀ ⊢ ∀'(#0 =' #0) := ⟨proof.eq_refl⟩
 
@@ -115,8 +131,9 @@ theorem rec_on {C : Π {m} (T : preTheory L m) (p : subformula L m 0), T ⊢ p �
   (imply₁ : ∀ {m} {T : preTheory L m} {p q}, C T (p ⟶ q ⟶ p) (axiomatic_classical_logic'.imply₁ p q))
   (imply₂ : ∀ {m} {T : preTheory L m} {p q r}, C T ((p ⟶ q ⟶ r) ⟶ (p ⟶ q) ⟶ p ⟶ r) (axiomatic_classical_logic'.imply₂ p q r))
   (contra : ∀ {m} {T : preTheory L m} {p q}, C T ((∼p ⟶ ∼q) ⟶ q ⟶ p) (axiomatic_classical_logic'.contraposition p q)) 
-  (specialize : ∀ {m} {T : preTheory L m} {p} {t}, C T (∀'p ⟶ subst t p) (specialize t))
+  (specialize : ∀ {m} {T : preTheory L m} {p} {t}, C T (∀'p ⟶ subst t p) (specialize p t))
   (dummy_univ : ∀ {m} {T : preTheory L m} {p q}, C T (∀'(dummy p ⟶ q) ⟶ p ⟶ ∀'q) (dummy_univ p q))
+  (non_empty : ∀ {T : preTheory L 0}, C T (∃'⊤) non_empty)
   (eq_refl : ∀ {T : preTheory L 0}, C T (∀'(#0 =' #0)) eq_refl)
   (eq_symm : ∀ {T : preTheory L 0}, C T (∀' ∀'((#0 =' #1) ⟶ (#1 =' #0))) eq_symm)
   (eq_trans : ∀ {T : preTheory L 0}, C T (∀' ∀' ∀'((#0 =' #1) ⟶ (#1 =' #2) ⟶ (#0 =' #2))) eq_trans)
@@ -135,6 +152,7 @@ begin
   case contra : m T p q { exact contra },
   case specialize : m T p t { exact specialize },
   case dummy_univ : m T p q { exact dummy_univ },
+  case non_empty { exact non_empty },
   case eq_refl : { exact eq_refl },
   case eq_symm : { exact eq_symm },
   case eq_trans : { exact eq_trans },
@@ -150,6 +168,7 @@ begin
   { intros m T p b IH U hyp, refine generalize (IH $ set.image_subset _ hyp) },
   { intros m T p q hyp_pq hyp_p IH₁ IH₂ U hyp, exact (IH₁ hyp) ⨀ (IH₂ hyp) },
   { intros m T p hyp_p U hyp, exact by_axiom (hyp hyp_p) },
+  { intros, simp },
   { intros, simp },
   { intros, simp },
   { intros, simp },
@@ -179,8 +198,9 @@ begin
   { rintros m T p q U r rfl, simp },
   { rintros m T p q r U s rfl, simp },
   { rintros m T p q U r rfl, simp },
-  { rintros m T p t U q rfl, refine hyp_right (specialize t) _ },
+  { rintros m T p t U q rfl, refine hyp_right (specialize p t) _ },
   { rintros m T p q U r rfl, refine hyp_right (dummy_univ p q) _ },
+  { simp },
   { simp },
   { simp },
   { simp },
@@ -238,12 +258,208 @@ begin
   { rintros T, refine ⟨[], by simp, by simp[empty_axiom]⟩ },
   { rintros T, refine ⟨[], by simp, by simp[empty_axiom]⟩ },
   { rintros T, refine ⟨[], by simp, by simp[empty_axiom]⟩ },
+  { rintros T, refine ⟨[], by simp, by simp[empty_axiom]⟩ },
   { rintros T p f, refine ⟨[], by simp, by simp[empty_axiom]⟩ },
   { rintros T p r, refine ⟨[], by simp, by simp[empty_axiom]⟩ },
 end
 
 instance : has_finite_character (formula L m) :=
 finite_character_of_finite_provable (formula L m) (λ T p, finite_character_aux)
+
+lemma exists_of_subst (p : subformula L m 1) (t) : T ⊢ subst t p ⟶ ∃' p :=
+contrapose.mp (imply_of_equiv
+  (show T ⊢ p.neg.fal ⟶ ∼subst t p, by simpa using specialize (∼p) t)
+  (iff_dn_refl_right $ ∀'∼p) (equiv_refl _))
+
+lemma specialize' {T} (p : subformula L m 1) : T ⊢ ∀' 𝗟 p ⟶ 𝗠 p :=
+by { have : T ⊢ ∀' 𝗟 p ⟶ subst &0 p.mlift, from specialize p.mlift &0, simpa using this }
+
+lemma use {p : subformula L m 1} (t) (h : T ⊢ subst t p) : T ⊢ ∃'p :=
+exists_of_subst p t ⨀ h
+
+@[simp] lemma forall_top : T ⊢ ∀'⊤ :=
+gen (by simp)
+
+@[simp] lemma non_empty' : T ⊢ ∃'⊤ :=
+by { cases m, { exact non_empty },
+  { have : T ⊢ subst &0 ⊤ ⟶ ∃'⊤, from exists_of_subst ⊤ &0,
+    simpa using this } }
+
+lemma forallK (p q) : T ⊢ ∀' (p ⟶ q) ⟶ ∀' p ⟶ ∀' q :=
+begin
+  have lmm₁ : T ⊢ ∀' (p ⟶ q) ⟶ ∀' (𝗗 (∀' p) ⟶ q),
+  { have : 𝗟'T +{ ∀'(𝗟 p ⟶ 𝗟 q) } ⊢ 𝗠 p ⟶ 𝗠 q, from deduction.mpr (by simpa using specialize' (p ⟶ q)),
+    have : 𝗟'T +{ ∀'(𝗟 p ⟶ 𝗟 q) } ⊢ ∀'𝗟 p ⟶ 𝗠 q, from imply_trans (specialize' _) this, 
+    refine deduction.mp (gen _), simp[preTheory.mlift_insert], exact this },
+  have lmm₂ : T ⊢ ∀' (𝗗 (∀'p) ⟶ q) ⟶ ∀' p ⟶ ∀' q, from dummy_univ (∀' p) q,
+  exact imply_trans lmm₁ lmm₂
+end
+
+lemma forall_of_equiv {p₁ p₂} (h : T ⊢ ∀' p₁) (hp : 𝗟'T ⊢ 𝗠 p₁ ⟷ 𝗠 p₂) : T ⊢ ∀' p₂ :=
+by { have : T ⊢ ∀'(p₁ ⟶ p₂), by simpa using generalize (iff_equiv.mp hp).1,
+     exact (forallK _ _) ⨀ this ⨀ h }
+
+lemma equiv_forall_of_equiv {p₁ p₂} (hp : 𝗟'T ⊢ 𝗠 p₁ ⟷ 𝗠 p₂) : T ⊢ ∀'p₁ ⟷ ∀'p₂ :=
+by { simp[iff_equiv], split,
+  { have : T ⊢ ∀'(p₁ ⟶ p₂), by simpa using generalize (iff_equiv.mp hp).1,
+    exact forallK _ _ ⨀ this },
+  { have : T ⊢ ∀'(p₂ ⟶ p₁), by simpa using generalize (iff_equiv.mp hp).2,
+    exact forallK _ _ ⨀ this } }
+
+lemma equiv_exists_of_equiv {p₁ p₂} (hp : 𝗟'T ⊢ 𝗠 p₁ ⟷ 𝗠 p₂) : T ⊢ ∃'p₁ ⟷ ∃'p₂ :=
+by simp[ex_def]; refine equiv_neg_of_equiv (equiv_forall_of_equiv (by simpa using equiv_neg_of_equiv hp))
+
+lemma univ_imply_dummy (p : subformula L m 1) (q : subformula L m 0) :
+  T ⊢ ∀'(p ⟶ 𝗗 q) ⟶ ∃'p ⟶ q :=
+begin
+  have : T ⊢ ∀'(∼𝗗 q ⟶ ∼p) ⟶ ∼q ⟶ ∀'∼p, by simpa using dummy_univ (∼q) (∼p),
+  refine imply_of_equiv this (equiv_forall_of_equiv (by simp)) (by simp[ex_def])
+end
+
+lemma exists_intro (p : subformula L m 1) (q : subformula L m 0)
+  (h : 𝗟'T ⊢ 𝗠 p ⟶ 𝗟 q) : T ⊢ ∃'p ⟶ q :=
+by { have : T ⊢ ∀'(p ⟶ 𝗗 q), by simpa using generalize h,
+     exact univ_imply_dummy p q ⨀ this }
+
+@[simp] lemma forall_bot : T ⊢ ∀'⊥ ⟷ ⊥ :=
+by { simp[iff_equiv],
+     have : T ⊢ ∼∀'∼⊤, by simp[←ex_def],
+     refine of_equiv (neg_of_equiv this (equiv_forall_of_equiv (by simp)))
+     (neg_iff (∀'⊥)) }
+
+@[simp] lemma forall_dummy (p : formula L m) : T ⊢ ∀'𝗗 p ⟷ p :=
+begin
+  simp[iff_equiv], split,
+  { have : T ⊢ ∀'(⊤ ⟶ 𝗗 p) ⟶ ∃'⊤ ⟶ p, from univ_imply_dummy ⊤ p,
+    refine imply_of_equiv this (equiv_forall_of_equiv $ by simp) (by simp) },
+  { refine deduction.mp (gen $ by simp) }
+end
+
+section prenex_normal_form
+
+lemma neg_forall_pnf (p) : T ⊢ ∼∀'p ⟷ ∃'∼p :=
+equiv_neg_of_equiv (equiv_forall_of_equiv (by simp[neg_eq]))
+
+lemma neg_exists_pnf (p) : T ⊢ ∼∃'p ⟷ ∀'∼p := by simp[ex_def]
+
+@[simp] lemma or_forall_pnf (p q) : T ⊢ (∀'p) ⊔ q ⟷ ∀'(p ⊔ 𝗗 q) :=
+begin
+  have lmm₁ : T ⊢ (∀'p) ⊔ q ⟶ ∀'(p ⊔ 𝗗 q),
+  { have : 𝗟'T ⊢ (∀'𝗟 p) ⊔ 𝗟 q ⟶ 𝗠 p ⊔ 𝗟 q,
+    { have : 𝗟'T ⊢ ∀'𝗟 p ⟶ 𝗠 p, from specialize' p,
+      exact or_imply (∀'𝗟 p) (𝗟 q) (𝗠 p ⊔ 𝗟 q) ⨀ (imply_trans this (by simp)) ⨀ (by simp) },
+    have : 𝗟'(T +{ (∀'p) ⊔ q }) ⊢ 𝗠 p ⊔ 𝗟 q, simpa using deduction.mpr this,
+    have : T +{ (∀'p) ⊔ q } ⊢ ∀'(p ⊔ 𝗗 q), by simpa using generalize this,
+    exact deduction.mp this },
+  have lmm₂ : T ⊢ ∀'(p ⊔ 𝗗 q) ⟶ (∀'p) ⊔ q,
+  { simp[has_sup.sup, subformula.or, imply_eq, neg_eq],
+    have : T ⊢ ∀'(∼p ⟶ 𝗗 q) ⟶ ∃'∼p ⟶ q, from univ_imply_dummy (∼p) q,
+    refine imply_of_equiv this (by simp) (equiv_imply_of_equiv (equiv_symm (neg_forall_pnf p)) (by simp)) },
+  refine iff_equiv.mpr ⟨lmm₁, lmm₂⟩
+end
+
+@[simp] lemma and_exists_pnf (p q) : T ⊢ (∃'p) ⊓ q ⟷ ∃'(p ⊓ 𝗗 q) :=
+begin
+  have : T ⊢ (∀'∼p) ⊔ ∼q ⟷ ∀'∼p ⊔ 𝗗 (∼q), from or_forall_pnf (∼p) (∼q),
+  refine equiv_of_equiv (equiv_neg_of_equiv this) _ _,
+  { show T ⊢ ∼((∀'∼p) ⊔ ∼q) ⟷ (∃'p) ⊓ q,
+    refine equiv_of_equiv (neg_or_equiv_and_neg (∀'∼p) (∼q))
+      (equiv_refl _) (equiv_and_of_equiv (equiv_refl _) (iff_dn_refl_left q)) },
+  { show T ⊢ ∼∀'(∼p ⊔ 𝗗 (∼q)) ⟷ ∃'(p ⊓ 𝗗 q),
+    refine equiv_neg_of_equiv (equiv_forall_of_equiv $ equiv_symm (by simp[neg_eq])) }
+end
+
+@[simp] lemma and_forall_pnf (p q) : T ⊢ (∀'p) ⊓ q ⟷ ∀'(p ⊓ 𝗗 q) :=
+begin
+  have lmm₁ : T ⊢ (∀'p) ⊓ q ⟶ ∀'(p ⊓ 𝗗 q),
+  { have : 𝗟'T ⊢ (∀'𝗟 p) ⊓ 𝗟 q ⟶ 𝗠 p ⊓ 𝗟 q,
+    { have : 𝗟'T ⊢ ∀'𝗟 p ⟶ 𝗠 p, from specialize' p,
+      exact imply_and ((∀'𝗟 p) ⊓ 𝗟 q) (𝗠 p) (𝗟 q) ⨀ (imply_trans (by simp) this) ⨀ (by simp) },
+    have : 𝗟'(T +{ (∀'p) ⊓ q }) ⊢ 𝗠 p ⊓ 𝗟 q, simpa using deduction.mpr this,
+    have : T +{ (∀'p) ⊓ q } ⊢ ∀'(p ⊓ 𝗗 q), by simpa using generalize this,
+    exact deduction.mp this },
+  have lmm₂ : T ⊢ ∀'(p ⊓ 𝗗 q) ⟶ (∀'p) ⊓ q,
+  { have lmm₃ : T ⊢ ∀'(p ⊓ 𝗗 q) ⟶ ∀'p, from forallK (p ⊓ 𝗗 q) p ⨀ (gen $ by simp),
+    have lmm₄ : T ⊢ ∀'(p ⊓ 𝗗 q) ⟶ q,
+    { have : T ⊢ ∀'(p ⊓ 𝗗 q) ⟶ ∀'𝗗 q, from forallK (p ⊓ 𝗗 q) (𝗗 q) ⨀ (gen $ by simp),
+      refine imply_trans this (equiv_mp (forall_dummy _)) },
+    refine imply_and (∀'(p ⊓ 𝗗 q)) (∀'p) q ⨀ lmm₃ ⨀ lmm₄ },
+  refine iff_equiv.mpr ⟨lmm₁, lmm₂⟩
+end
+
+@[simp] lemma or_exists_pnf (p q) : T ⊢ (∃'p) ⊔ q ⟷ ∃'(p ⊔ 𝗗 q) :=
+begin
+  have : T ⊢ (∀'∼p) ⊓ ∼q ⟷ ∀'∼p ⊓ 𝗗 (∼q), from and_forall_pnf (∼p) (∼q),
+  have := equiv_neg_of_equiv this,
+  refine equiv_of_equiv this _ _,
+  { show T ⊢ ∼((∀'∼p) ⊓ ∼q) ⟷ (∃'p) ⊔ q,
+    refine equiv_of_equiv (neg_and_equiv_or_neg (∀'∼p) (∼q))
+      (equiv_refl _) (equiv_or_of_equiv (equiv_refl _) (iff_dn_refl_left q)) },
+  { show T ⊢ ∼∀'(∼p ⊓ 𝗗 (∼q)) ⟷ ∃'(p ⊔ 𝗗 q),
+    refine equiv_neg_of_equiv (equiv_forall_of_equiv $ equiv_symm (by simp[neg_eq])) }
+end
+
+lemma imply_forall_pnf (p q) : T ⊢ (p ⟶ ∀'q) ⟷ ∀'(𝗗 p ⟶ q) :=
+by { have : T ⊢ ((∀'q) ⊔ ∼p) ⟷ ∀'(q ⊔ ∼𝗗 p), by simpa using or_forall_pnf q ∼p,
+     exact equiv_of_equiv this (equiv_symm (by simp))
+       (equiv_forall_of_equiv (equiv_symm (by simp))) }
+
+lemma imply_exists_pnf (p q) : T ⊢ (p ⟶ ∃'q) ⟷ ∃'(𝗗 p ⟶ q) :=
+by{ have : T ⊢ ((∃'q) ⊔ ∼p) ⟷ ∃'(q ⊔ ∼𝗗 p), by simpa using or_exists_pnf q ∼p,
+    refine equiv_of_equiv this (equiv_symm impl_iff_or')
+      (equiv_exists_of_equiv $ equiv_symm $ by simp)}
+
+lemma exists_imply_pnf (p q) : T ⊢ (∃'p ⟶ q) ⟷ ∀'(p ⟶ 𝗗 q) :=
+by{ have : T ⊢ ((∀'∼p) ⊔ q) ⟷ ∀'(∼p ⊔ 𝗗 q), by simp,
+    refine equiv_of_equiv this _ _,
+    { have : T ⊢ (∼∼∀'∼p) ⊔ q ⟷ ∃'p ⟶ q, from equiv_symm (by simp[ex_def]),
+      refine equiv_trans (equiv_or_of_equiv _ _) this; simp },
+    { refine equiv_forall_of_equiv (equiv_symm $ by simp) } }
+
+lemma forall_imply_pnf (p q) : T ⊢ (∀'p ⟶ q) ⟷ ∃'(p ⟶ 𝗗 q) :=
+by{ have : T ⊢ ((∃'∼p) ⊔ q) ⟷ ∃'(∼p ⊔ 𝗗 q), by simp,
+    refine equiv_of_equiv this _ _,
+    { have : T ⊢ (∃'∼p) ⊔ q ⟷ ∀'∼∼p ⟶ q, from equiv_symm (by simp[ex_def]),
+      refine equiv_trans this (equiv_imply_of_equiv (equiv_forall_of_equiv _) _); simp },
+    { refine equiv_exists_of_equiv (equiv_symm $ by simp) } }
+
+lemma forall_imply_forall_pnf (p q) : T ⊢ (∀'p ⟶ ∀'q) ⟷ ∃' ∀'(𝗡 𝗗 𝗠 p ⟶ 𝗗 q) :=
+begin
+  have : 𝗟'T ⊢ (𝗠 p ⟶ ∀'𝗟 q) ⟷ ∀'(𝗗 𝗠 p ⟶ 𝗟 q), from imply_forall_pnf (𝗠 p) (𝗟 q),
+  have lmm₁ : T ⊢ ∃'(p ⟶ ∀' 𝗗 q) ⟷ ∃' ∀'(𝗡 𝗗 𝗠 p ⟶ 𝗗 q),
+    from equiv_exists_of_equiv (by simpa using this),
+  have lmm₂ : T ⊢ (∀'p ⟶ ∀'q) ⟷ ∃'(p ⟶ ∀' 𝗗 q), by simpa using forall_imply_pnf p (∀'q),
+  exact equiv_trans lmm₂ lmm₁
+end
+
+lemma forall_imply_exists_pnf (p q) : T ⊢ (∀'p ⟶ ∃'q) ⟷ ∃' ∃'(𝗡 𝗗 𝗠 p ⟶ 𝗗 q) :=
+begin
+  have : 𝗟'T ⊢ (𝗠 p ⟶ ∃'𝗟 q) ⟷ ∃'(𝗗 𝗠 p ⟶ 𝗟 q), from imply_exists_pnf (𝗠 p) (𝗟 q),
+  have lmm₁ : T ⊢ ∃'(p ⟶ ∃' 𝗗 q) ⟷ ∃' ∃'(𝗡 𝗗 𝗠 p ⟶ 𝗗 q),
+    from equiv_exists_of_equiv (by simpa using this),
+  have lmm₂ : T ⊢ (∀'p ⟶ ∃'q) ⟷ ∃'(p ⟶ ∃' 𝗗 q), by simpa using forall_imply_pnf p (∃'q),
+  exact equiv_trans lmm₂ lmm₁
+end
+
+lemma exists_imply_forall_pnf (p q) : T ⊢ (∃'p ⟶ ∀'q) ⟷ ∀' ∀'(𝗡 𝗗 𝗠 p ⟶ 𝗗 q) :=
+begin
+  have : 𝗟'T ⊢ (𝗠 p ⟶ ∀'𝗟 q) ⟷ ∀'(𝗗 𝗠 p ⟶ 𝗟 q), from imply_forall_pnf (𝗠 p) (𝗟 q),
+  have lmm₁ : T ⊢ ∀'(p ⟶ ∀' 𝗗 q) ⟷ ∀' ∀'(𝗡 𝗗 𝗠 p ⟶ 𝗗 q),
+    from equiv_forall_of_equiv (by simpa using this),
+  have lmm₂ : T ⊢ (∃'p ⟶ ∀'q) ⟷ ∀'(p ⟶ ∀' 𝗗 q), by simpa using exists_imply_pnf p (∀'q),
+  exact equiv_trans lmm₂ lmm₁
+end
+
+lemma exists_imply_exists_pnf (p q) : T ⊢ (∃'p ⟶ ∃'q) ⟷ ∀' ∃'(𝗡 𝗗 𝗠 p ⟶ 𝗗 q) :=
+begin
+  have : 𝗟'T ⊢ (𝗠 p ⟶ ∃'𝗟 q) ⟷ ∃'(𝗗 𝗠 p ⟶ 𝗟 q), from imply_exists_pnf (𝗠 p) (𝗟 q),
+  have lmm₁ : T ⊢ ∀'(p ⟶ ∃' 𝗗 q) ⟷ ∀' ∃'(𝗡 𝗗 𝗠 p ⟶ 𝗗 q),
+    from equiv_forall_of_equiv (by simpa using this),
+  have lmm₂ : T ⊢ (∃'p ⟶ ∃'q) ⟷ ∀'(p ⟶ ∃' 𝗗 q), by simpa using exists_imply_pnf p (∃'q),
+  exact equiv_trans lmm₂ lmm₁
+end
+
+end prenex_normal_form
 
 end provable
 
