src/QL/FOL/pnf.lean
@@ -1,0 +1,243 @@
+import QL.FOL.deduction
+
+-- Prenex normal form
+
+universes u v
+
+namespace fol
+open_locale logic_symbol
+open subformula
+
+variables (L : language.{u}) (m n : ℕ)
+
+inductive pnf (m : ℕ) : ℕ → Type u
+| openformula {n} : Π p : subformula L m n, p.is_open → pnf n
+| fal         {n} : pnf (n + 1) → pnf n
+| ex          {n} : pnf (n + 1) → pnf n
+
+variables {L m n}
+
+instance : has_univ_quantifier' (pnf L m) := ⟨@pnf.fal L m⟩
+
+instance : has_exists_quantifier' (pnf L m) := ⟨@pnf.ex L m⟩
+
+namespace pnf
+
+@[simp] def to_formula : Π {n}, pnf L m n → subformula L m n
+| n (openformula p hp) := p
+| n (fal φ)            := ∀'to_formula φ
+| n (ex  φ)            := ∃'to_formula φ
+
+instance : has_coe (pnf L m n) (subformula L m n) := ⟨@to_formula L m n⟩
+
+@[simp] def neg : Π {n}, pnf L m n → pnf L m n
+| n (openformula p hp) := openformula (∼p) (by simpa[is_open] using hp)
+| n (fal φ)            := ∃'φ.neg
+| n (ex φ)             := ∀'φ.neg
+
+@[simp] def imply : Π {n}, pnf L m n → pnf L m n → pnf L m n
+| n (openformula p hp) (openformula q hq) := openformula (p ⟶ q) (by simp; exact ⟨hp, hq⟩)
+| n (openformula p hp) (fal φ)            := ∃'φ.neg
+| n (openformula p hp) (ex φ)             := ∀'φ.neg
+
+
+#check 0
+/--/
+
+
+
+#check 0
+/-
+
+@[simp] def rank : pnf L → ℕ := λ p, p.1.length
+
+def rew (s : ℕ → term L) : pnf L → pnf L
+| ⟨Q, p, h⟩ := ⟨Q, p.rew (s^Q.length), by simp[h]⟩
+
+instance : has_pow (pnf L) ℕ := ⟨λ p i, p.rew (λ x, #(x + i))⟩
+
+@[simp] lemma rew_to_formula_eq_to_formula_rew : ∀ (p : pnf L) (s : ℕ → term L),
+  (p.rew s).to_formula = p.to_formula.rew s
+| ⟨[], p, h⟩     s := by simp[rew]
+| ⟨𝚷 :: Q, p, h⟩ s := by simp[rew, ←rew_to_formula_eq_to_formula_rew ⟨Q, p, by simp[h]⟩ (s^1),
+    rewriting_sf_itr.pow_add, show 1 + Q.length = Q.length + 1, from add_comm _ _]
+| ⟨𝚺 :: Q, p, h⟩ s := by simp[rew, ←rew_to_formula_eq_to_formula_rew ⟨Q, p, by simp[h]⟩ (s^1),
+    rewriting_sf_itr.pow_add, show 1 + Q.length = Q.length + 1, from add_comm _ _]
+
+@[simp] lemma pow_to_formula_eq_to_formula_pow (p : pnf L) (i : ℕ) : (p^i).to_formula = p.to_formula^i :=
+by simp[formula.pow_eq, rew_to_formula_eq_to_formula_rew, has_pow.pow]
+
+lemma rew_fal (Q : list bool) (p : formula L) {h} (s : ℕ → term L) :
+  (⟨(𝚷 :: Q), p, h⟩ : pnf L).rew s = ∀.(⟨Q, p, h⟩ : pnf L).rew (s^1) :=
+by simp[rew, show Q.length + 1 = 1 + Q.length, from add_comm _ _, rewriting_sf_itr.pow_add]
+
+@[simp] lemma rew_fal' : ∀ (p : pnf L) (s : ℕ → term L),
+  (∀.p : pnf L).rew s = ∀.(p.rew (s^1))
+| ⟨Q, p, h⟩ s := by simp[rew_fal]
+
+lemma rew_ex (Q : list bool) (p : formula L) {h} (s : ℕ → term L) :
+  (⟨(𝚺 :: Q), p, h⟩ : pnf L).rew s = ∃.(⟨Q, p, h⟩ : pnf L).rew (s^1) :=
+by simp[rew, show Q.length + 1 = 1 + Q.length, from add_comm _ _, rewriting_sf_itr.pow_add]
+
+@[simp] lemma rew_ex' : ∀ (p : pnf L) (s : ℕ → term L),
+  (∃.p : pnf L).rew s = ∃.(p.rew (s^1))
+| ⟨Q, p, h⟩ s := by simp[rew_ex]
+
+lemma nested_rew (p : pnf L) (s₀ s₁) :
+  (p.rew s₀).rew s₁ = p.rew (λ x, (s₀ x).rew s₁) :=
+to_formula_inj.mp (by simp[formula.nested_rew])
+
+@[simp] lemma rew_rank : ∀ (p : pnf L) (s), (p.rew s).rank = p.rank
+| ⟨[], p, h⟩     s := by simp[rew]
+| ⟨𝚷 :: Q, p, h⟩ s := by simp[rew]
+| ⟨𝚺 :: Q, p, h⟩ s := by simp[rew]
+
+@[simp] lemma pow_rank (p : pnf L) (i : ℕ) : (p^i).rank = p.rank :=
+by simp[has_pow.pow]
+
+@[simp] def neg : pnf L → pnf L
+| ⟨[], p, h⟩ := ⟨[], ∼p, by simp[h]⟩
+| ⟨𝚷 :: Q, p, h⟩ := ∃.neg ⟨Q, p, by simp[h]⟩
+| ⟨𝚺 :: Q, p, h⟩ := ∀.neg ⟨Q, p, by simp[h]⟩
+using_well_founded {rel_tac := λ _ _, `[exact ⟨_, measure_wf rank⟩]}
+
+instance : has_negation (pnf L) := ⟨neg⟩
+
+@[simp] def imply : pnf L → pnf L → pnf L
+| ⟨[], p₁, h₁⟩      ⟨[], p₂, h₂⟩      := ⟨[], p₁ ⟶ p₂, by simp[h₁, h₂]⟩
+| ⟨[], p₁, h₁⟩      ⟨𝚷 :: Q₂, p₂, h₂⟩ := ∀.imply (⟨[], p₁^1, by simp[h₁]⟩) ⟨Q₂, p₂, h₂⟩
+| ⟨[], p₁, h₁⟩      ⟨𝚺 :: Q₂, p₂, h₂⟩ := ∃.imply ⟨[], p₁^1, by simp[h₁]⟩ ⟨Q₂, p₂, h₂⟩
+| ⟨𝚷 :: Q₁, p₁, h₁⟩ ⟨[], p₂, h₂⟩      := ∃.imply ⟨Q₁, p₁, by simp[h₁]⟩ ⟨[], p₂^1, by simp[h₂]⟩
+| ⟨𝚷 :: Q₁, p₁, h₁⟩ ⟨𝚷 :: Q₂, p₂, h₂⟩ :=
+    ∃.(∀.imply (pnf.mk Q₁ p₁ h₁^1) ((pnf.mk Q₂ p₂ (by simp[h₂])).rew ı-{1}) : pnf L)
+| ⟨𝚷 :: Q₁, p₁, h₁⟩ ⟨𝚺 :: Q₂, p₂, h₂⟩ :=
+    ∃.(∃.imply (pnf.mk Q₁ p₁ h₁^1) ((pnf.mk Q₂ p₂ (by simp[h₂])).rew ı-{1}) : pnf L)
+| ⟨𝚺 :: Q₁, p₁, h₁⟩ ⟨[], p₂, h₂⟩      := ∀.imply ⟨Q₁, p₁, by simp[h₁]⟩ ⟨[], p₂^1, by simp[h₂]⟩
+| ⟨𝚺 :: Q₁, p₁, h₁⟩ ⟨𝚷 :: Q₂, p₂, h₂⟩ :=
+    ∀.(∀.imply (pnf.mk Q₁ p₁ h₁^1) ((pnf.mk Q₂ p₂ (by simp[h₂])).rew ı-{1}) : pnf L)
+| ⟨𝚺 :: Q₁, p₁, h₁⟩ ⟨𝚺 :: Q₂, p₂, h₂⟩ :=
+    ∀.(∃.imply (pnf.mk Q₁ p₁ h₁^1) ((pnf.mk Q₂ p₂ (by simp[h₂])).rew ı-{1}) : pnf L)
+using_well_founded {rel_tac := λ _ _, `[exact ⟨_, measure_wf (λ x, x.fst.rank + x.snd.rank)⟩]}
+
+instance : has_arrow (pnf L) := ⟨imply⟩
+
+end pnf
+
+namespace formula
+
+@[simp] def to_pnf : formula L → pnf L
+| ⊤         := ⟨[], ⊤, by simp⟩
+| (app p v) := ⟨[], app p v, by simp⟩
+| ((t : term L) =' u) := ⟨[], (t : term L) =' u, by simp⟩
+| (p ⟶ q) := (to_pnf p).imply (to_pnf q)
+| (∼p) := (to_pnf p).neg
+| (∀.(p : formula L)) := ∀.(to_pnf p)
+
+end formula
+
+lemma equiv_normalize_imply : ∀ (p q : pnf L) (T : Theory L),
+  (p.imply q).to_formula  ≈[T] p.to_formula ⟶ q.to_formula
+| ⟨[], p₁, h₁⟩      ⟨[], p₂, h₂⟩      T := by simp
+| ⟨[], p₁, h₁⟩      ⟨𝚷 :: Q₂, p₂, h₂⟩ T := by { simp, have ih := equiv_normalize_imply ⟨[], p₁^1, by simp[h₁]⟩ ⟨Q₂, p₂, h₂⟩,
+    calc     ∀.((pnf.mk ([]) (p₁^1) (by simp[h₁])).imply (pnf.mk Q₂ p₂ h₂)).to_formula
+        ≈[(T)] ∀.((pnf.mk ([]) (p₁^1) (by simp[h₁])).to_formula ⟶ (pnf.mk Q₂ p₂ h₂).to_formula)
+    : show _ ≈[T] _, from provable.equiv_univ_of_equiv (ih _)
+    ... ≈[T] p₁ ⟶ ∀.(pnf.mk Q₂ p₂ h₂).to_formula
+    : by { symmetry, refine by simp[classical_logic.equiv] } }
+| ⟨[], p₁, h₁⟩      ⟨𝚺 :: Q₂, p₂, h₂⟩ T := by { simp, have ih := equiv_normalize_imply ⟨[], p₁^1, by simp[h₁]⟩ ⟨Q₂, p₂, h₂⟩,
+    calc     ∃.((pnf.mk ([]) (p₁^1) (by simp[h₁])).imply (pnf.mk Q₂ p₂ h₂)).to_formula
+        ≈[T] ∃.((pnf.mk ([]) (p₁^1) (by simp[h₁])).to_formula ⟶ (pnf.mk Q₂ p₂ h₂).to_formula)
+    : show _ ≈[T] _, from provable.equiv_ex_of_equiv (ih _)
+    ... ≈[T] p₁ ⟶ ∃.(pnf.mk Q₂ p₂ h₂).to_formula
+    : by { symmetry, simp[classical_logic.equiv] } }
+| ⟨𝚷 :: Q₁, p₁, h₁⟩ ⟨[], p₂, h₂⟩      T := by { simp, have ih := equiv_normalize_imply ⟨Q₁, p₁, h₁⟩ (pnf.mk ([]) p₂ h₂^1),
+    calc     ∃.((pnf.mk Q₁ p₁ h₁).imply (pnf.mk ([]) p₂ h₂^1)).to_formula
+        ≈[T] ∃.((pnf.mk Q₁ p₁ h₁).to_formula ⟶ (pnf.mk ([]) p₂ h₂^1).to_formula)
+    : show _ ≈[T] _, from provable.equiv_ex_of_equiv (ih _)
+    ... ≈[T] ∀.(pnf.mk Q₁ p₁ (by simp[h₁])).to_formula ⟶ p₂
+    : by { symmetry, simp[classical_logic.equiv] } }
+| ⟨𝚷 :: Q₁, p₁, h₁⟩ ⟨𝚷 :: Q₂, p₂, h₂⟩ T := by { simp,
+    have ih := equiv_normalize_imply (pnf.mk Q₁ p₁ h₁^1) ((pnf.mk Q₂ p₂ h₂).rew ı-{1}),
+    calc     ∃.∀.((pnf.mk Q₁ p₁ h₁^1).imply ((pnf.mk Q₂ p₂ h₂).rew ı-{1})).to_formula
+        ≈[T] ∃.∀.((pnf.mk Q₁ p₁ h₁^1).to_formula ⟶ ((pnf.mk Q₂ p₂ h₂).rew ı-{1}).to_formula)
+    : show _ ≈[T] _, from provable.equiv_ex_of_equiv (provable.equiv_univ_of_equiv (ih _))
+    ... ≈[T] ∃.((pnf.mk Q₁ p₁ h₁).to_formula ⟶ (∀.(pnf.mk Q₂ p₂ h₂).to_formula)^1)
+    : by { show _ ≈[T] _, symmetry, simp[classical_logic.equiv, formula.fal_pow_discard],
+           refine provable.equiv_ex_of_equiv (by simp) }
+    ... ≈[T] ∀.(pnf.mk Q₁ p₁ h₁).to_formula ⟶ ∀.(pnf.mk Q₂ p₂ h₂).to_formula
+    : by { symmetry, simp [classical_logic.equiv] } }
+| ⟨𝚷 :: Q₁, p₁, h₁⟩ ⟨𝚺 :: Q₂, p₂, h₂⟩ T := by { simp, 
+    have ih := equiv_normalize_imply (pnf.mk Q₁ p₁ h₁^1) ((pnf.mk Q₂ p₂ h₂).rew ı-{1}),
+    calc     ∃.∃.((pnf.mk Q₁ p₁ h₁^1).imply ((pnf.mk Q₂ p₂ h₂).rew ı-{1})).to_formula
+        ≈[T] ∃.∃.((pnf.mk Q₁ p₁ h₁^1).to_formula ⟶ ((pnf.mk Q₂ p₂ h₂).rew ı-{1}).to_formula)
+    : show _ ≈[T] _, from provable.equiv_ex_of_equiv (provable.equiv_ex_of_equiv (ih _))
+    ... ≈[T] ∃.((pnf.mk Q₁ p₁ h₁).to_formula ⟶ (∃.(pnf.mk Q₂ p₂ h₂).to_formula)^1)
+    : by { show _ ≈[T] _, symmetry, simp[classical_logic.equiv, formula.ex_pow_discard],
+           refine provable.equiv_ex_of_equiv (by simp) }
+    ... ≈[T] ∀.(pnf.mk Q₁ p₁ h₁).to_formula ⟶ ∃.(pnf.mk Q₂ p₂ h₂).to_formula
+    : by { symmetry, simp [classical_logic.equiv] } }
+| ⟨𝚺 :: Q₁, p₁, h₁⟩ ⟨[], p₂, h₂⟩      T := by { simp, have ih := equiv_normalize_imply ⟨Q₁, p₁, h₁⟩ (pnf.mk ([]) p₂ h₂^1),
+    calc     ∀.((pnf.mk Q₁ p₁ h₁).imply (pnf.mk ([]) p₂ h₂^1)).to_formula
+        ≈[T] ∀.((pnf.mk Q₁ p₁ h₁).to_formula ⟶ (pnf.mk ([]) p₂ h₂^1).to_formula)
+    : show _ ≈[T] _, from provable.equiv_univ_of_equiv (ih _)
+    ... ≈[T] ∃.(pnf.mk Q₁ p₁ (by simp[h₁])).to_formula ⟶ p₂
+    : by { symmetry, simp[classical_logic.equiv] } }
+| ⟨𝚺 :: Q₁, p₁, h₁⟩ ⟨𝚷 :: Q₂, p₂, h₂⟩ T := by { simp,
+    have ih := equiv_normalize_imply (pnf.mk Q₁ p₁ h₁^1) ((pnf.mk Q₂ p₂ h₂).rew ı-{1}),
+    calc     ∀.∀.((pnf.mk Q₁ p₁ h₁^1).imply ((pnf.mk Q₂ p₂ h₂).rew ı-{1})).to_formula
+        ≈[T] ∀.∀.((pnf.mk Q₁ p₁ h₁^1).to_formula ⟶ ((pnf.mk Q₂ p₂ h₂).rew ı-{1}).to_formula)
+    : show _ ≈[T] _, from provable.equiv_univ_of_equiv (provable.equiv_univ_of_equiv (ih _))
+    ... ≈[T] ∀.((pnf.mk Q₁ p₁ h₁).to_formula ⟶ (∀.(pnf.mk Q₂ p₂ h₂).to_formula)^1)
+    : by { show _ ≈[T] _, symmetry, simp[classical_logic.equiv, formula.fal_pow_discard],
+           refine provable.equiv_univ_of_equiv (by simp) }
+    ... ≈[T] ∃.(pnf.mk Q₁ p₁ h₁).to_formula ⟶ ∀.(pnf.mk Q₂ p₂ h₂).to_formula
+    : by { symmetry, simp [classical_logic.equiv] } }
+| ⟨𝚺 :: Q₁, p₁, h₁⟩ ⟨𝚺 :: Q₂, p₂, h₂⟩ T := by { simp, 
+    have ih := equiv_normalize_imply (pnf.mk Q₁ p₁ h₁^1) ((pnf.mk Q₂ p₂ h₂).rew ı-{1}),
+    calc     ∀.∃.((pnf.mk Q₁ p₁ h₁^1).imply ((pnf.mk Q₂ p₂ h₂).rew ı-{1})).to_formula
+        ≈[T] ∀.∃.((pnf.mk Q₁ p₁ h₁^1).to_formula ⟶ ((pnf.mk Q₂ p₂ h₂).rew ı-{1}).to_formula)
+    : show _ ≈[T] _, from provable.equiv_univ_of_equiv (provable.equiv_ex_of_equiv (ih _))
+    ... ≈[T] ∀.((pnf.mk Q₁ p₁ h₁).to_formula ⟶ (∃.(pnf.mk Q₂ p₂ h₂).to_formula)^1)
+    : by { show _ ≈[T] _, symmetry, simp[classical_logic.equiv, formula.ex_pow_discard],
+           refine provable.equiv_univ_of_equiv (by simp) }
+    ... ≈[T] ∃.(pnf.mk Q₁ p₁ h₁).to_formula ⟶ ∃.(pnf.mk Q₂ p₂ h₂).to_formula
+    : by { symmetry, simp [classical_logic.equiv] } }
+using_well_founded {rel_tac := λ _ _, `[exact ⟨_, measure_wf (λ x, x.1.rank + x.2.1.rank)⟩]}
+
+lemma equiv_normalize_neg : ∀ (p : pnf L) (T : Theory L) , T ⊢ p.neg.to_formula ⟷ ∼p.to_formula
+| ⟨[], p, h⟩     T := by simp
+| ⟨𝚷 :: Q, p, h⟩ T := by simp;
+    calc ∃.(pnf.mk Q p (by simp[h])).neg.to_formula ≈[T] ∃.∼(pnf.mk Q p (by simp[h])).to_formula
+    : show _ ≈[T] _, from provable.equiv_ex_of_equiv (equiv_normalize_neg ⟨Q, p, by simp[h]⟩ _)
+                                                 ... ≈[T] ∼∀.(pnf.mk Q p (by simp[h])).to_formula
+    : classical_logic.equiv_neg_of_equiv (provable.equiv_univ_of_equiv (by simp))
+| ⟨𝚺 :: Q, p, h⟩ T := by { simp,
+    calc     ∀.(pnf.mk Q p (by simp[h])).neg.to_formula ≈[T] ∀.∼(pnf.mk Q p (by simp[h])).to_formula
+    : show _ ≈[T] _, from provable.equiv_univ_of_equiv (equiv_normalize_neg ⟨Q, p, by simp[h]⟩ _)
+                                                    ... ≈[T] ∼∃.(pnf.mk Q p (by simp[h])).to_formula
+    : by { simp[has_exists_quantifier.ex, formula.ex, classical_logic.equiv] } }
+
+@[reducible] def formula.normalize (p : formula L) : formula L := p.to_pnf.to_formula
+
+@[reducible] def formula.open (p : formula L) : formula L := p.to_pnf.2
+
+@[simp] lemma formula.open_is_open (p : formula L) : p.open.is_open := p.to_pnf.is_openform
+
+open axiomatic_classical_logic'
+
+lemma equiv_normalize : ∀ (p : formula L) {T : Theory L},  T ⊢ p ⟷ p.normalize
+| ⊤                 T := by simp[formula.normalize]
+| (formula.app p v) T := by simp[formula.normalize]
+| (t =' u)          T := by simp[formula.normalize]
+| (p ⟶ q)          T :=
+    by { simp[formula.normalize], 
+         have : T ⊢ p ⟶ q ⟷ (p.to_pnf.to_formula ⟶ q.to_pnf.to_formula) :=  (equiv_imply_of_equiv (equiv_normalize p) (equiv_normalize q)),
+         refine equiv_trans this (classical_logic.equiv_symm (equiv_normalize_imply p.to_pnf q.to_pnf T)) }
+| (∼p)              T := by { simp[formula.normalize],
+    have : T ⊢ ∼p ⟷ ∼p.to_pnf.to_formula, from equiv_neg_of_equiv (equiv_normalize p),
+    exact equiv_trans this (equiv_symm (equiv_normalize_neg p.to_pnf T)) }
+| (∀.p)           T := by { simp[formula.normalize], refine provable.equiv_univ_of_equiv (equiv_normalize p) }
+
+def formula.rank (p : formula L) : ℕ := p.to_pnf.rank
+
+end fol
